Fix following merge

compiler/backend/bvl_constScript.sml
@@ -203,17 +203,17 @@ QED
 end
 
 
-
 Definition dest_EqualInt_def:
-  dest_EqualInt (EqualInt i) = SOME i ∧
+  dest_EqualInt (EqualConst (Int i)) = SOME i ∧
   dest_EqualInt _ = NONE
 End
 
 Theorem dest_EqualInt_pmatch:
-  dest_EqualInt x = case x of EqualInt i => SOME i | _ => NONE
+  dest_EqualInt x = case x of EqualConst (Int i) => SOME i | _ => NONE
 Proof
   CONV_TAC(RAND_CONV patternMatchesLib.PMATCH_ELIM_CONV)
   \\ Cases_on ‘x’ \\ EVAL_TAC
+  \\ rename [‘EqualConst cc’] \\ Cases_on ‘cc’ \\ EVAL_TAC
 QED
 
 Definition SmartOp1_def:
