compiler/backend/semantics/closSemScript.sml
@@ -297,8 +297,10 @@ Definition do_app_def:
         Rval (Boolv (LENGTH xs = l),s)
     | (TagLenEq n l,[Block tag xs]) =>
         Rval (Boolv (tag = n ∧ LENGTH xs = l),s)
-    | (EqualInt i,[Number j]) =>
-        Rval (Boolv (i = j), s)
+    | (EqualConst p,[x1]) =>
+        (case p of
+         | Int i => (case x1 of Number j => Rval (Boolv (i = j), s) | _ => Error)
+         | _ => Error)
     | (Equal,[x1;x2]) =>
         (case do_eq x1 x2 of
          | Eq_val b => Rval (Boolv b, s)
